proof/SimProgUnified.v
@@ -1,0 +1,111 @@
+Require Import Events.
+Require Import Values.
+Require Import AST.
+Require Import Memory.
+Require Import Globalenvs.
+Require Import Smallstep.
+Require Import CoqlibC.
+Require Import Skeleton.
+Require Import ModSem.
+Require Import SimSymb.
+Require Import Integers.
+Require Import ASTC.
+Require Import Maps.
+Require Import LinkingC.
+
+Require Import Syntax Sem Mod ModSem.
+Require Import SimMem SimModSemUnified SimModUnified.
+Require Import Sound SemProps.
+
+Set Implicit Arguments.
+
+
+
+
+
+Module ProgPair.
+Section PROGPAIR.
+Context `{SMOS: SimMemOhs.class} {SS: SimSymb.class SM} {SU: Sound.class}.
+
+  Definition t := list ModPair.t.
+
+  Definition sim (pp: t) := List.Forall ModPair.sim pp.
+
+  Definition src (pp: t): program := List.map ModPair.src pp.
+  Definition tgt (pp: t): program := List.map ModPair.tgt pp.
+
+  (* Definition ss_link (pp: t): option SimSymb.t := link_list (List.map ModPair.ss pp). *)
+  (* ############ TODO: *)
+  (* ModPair.wf mp0 /\ ModPair.wf mp1 /\ link mp0.(src) mp1.(src) = Some /\ link mp1.(tgt) mp1.(tgt) = Some *)
+  (* =================> link mp0.(ss) mp1.(ss) suceeds. *)
+  (* Move ModPair.wf into SimSymb and obligate its proof? *)
+
+End PROGPAIR.
+End ProgPair.
+
+Hint Unfold ProgPair.sim ProgPair.src ProgPair.tgt.
+(* Hint Unfold ProgPair.ss_link. *)
+
+
+
+
+
+
+Section SIM.
+Context `{SMOS: SimMemOhs.class} {SS: SimSymb.class SM} {SU: Sound.class}.
+
+  Variable pp: ProgPair.t.
+  Hypothesis SIMPROG: ProgPair.sim pp.
+  Let p_src := (ProgPair.src pp).
+  Let p_tgt := (ProgPair.tgt pp).
+
+
+
+  Theorem sim_link_sk
+          sk_link_src
+          (LOADSRC: (link_sk p_src) = Some sk_link_src)
+          (WF: forall md, In md p_src -> <<WF: Sk.wf md>>):
+      exists ss_link sk_link_tgt,
+        <<LOADTGT: (link_sk p_tgt) = Some sk_link_tgt>>
+        /\ <<SIMSK: SimSymb.wf ss_link>>
+        /\ <<SKSRC: ss_link.(SimSymb.src) = sk_link_src>>
+        /\ <<SKTGT: ss_link.(SimSymb.tgt) = sk_link_tgt>>
+        /\ <<LE: Forall (fun mp => (SimSymb.le mp.(ModPair.ss) ss_link)) pp>>.
+  Proof.
+    u. subst_locals. ginduction pp; ii; ss. destruct a; ss.
+    unfold ProgPair.src in *. unfold link_sk in *. ss. destruct (classic (t = [])).
+    { clarify; ss. cbn in *. clarify. clear IHt. inv SIMPROG. inv H2. inv H1. ss.
+      esplits; eauto. econs; eauto. ss. refl.
+    }
+    rename H into NNIL. eapply link_list_cons_inv in LOADSRC; cycle 1.
+    { destruct t; ss. }
+    des. rename sk_link_src into sk_link_link_src. rename restl into sk_link_src.
+    inv SIMPROG. exploit IHt; eauto. intro IH; des.
+    inv H1. ss. exploit (SimSymb.wf_link).
+    3: { rewrite SKSRC. eapply HD. }
+    all: eauto.
+    { rewrite SKSRC. eapply WF; et. }
+    { eapply link_list_preserves_wf_sk; eauto. }
+    { eapply SimSymb.wf_preserves_wf; et. rewrite SKSRC. eapply WF; et. }
+    { eapply SimSymb.wf_preserves_wf; et. eapply link_list_preserves_wf_sk; eauto. }
+    i; des. esplits; eauto.
+    - eapply link_list_cons; eauto.
+      rewrite SKTGT in LINKTGT. ss.
+    - econs; eauto. rewrite Forall_forall in *. ii.
+      all ltac:(fun H => apply link_list_linkorder in H). des.
+      rewrite Forall_forall in *. etrans; eauto.
+  Qed.
+
+End SIM.
+
+
+
+
+
+
+
+
+
+
+
+
